Finish the tau case

proofmode/HPSim.v
@@ -21,6 +21,31 @@ Require Import ProofMode Invariant.
 
 Require Import HTactics.
 
+
+
+
+
+  Lemma URA_wf_extends_add `{Σ: GRA.t} (r r' c: Σ)
+    (EXT : URA.extends r r')
+    (WF : URA.wf (r' ⋅ c))
+    :
+    URA.wf (r ⋅ c).
+  Proof.
+    eapply URA.wf_extends; eauto.
+    eapply URA.extends_add. eauto.
+  Qed.
+
+  Lemma URA_extends_refl `{Σ: GRA.t} (r: Σ):
+    URA.extends r r.
+  Proof. refl. Qed.
+
+
+
+
+
+  
+
+
 Section HPSIM.
 
   Context `{Σ: GRA.t}.
@@ -33,9 +58,9 @@ Section HPSIM.
     fun fmr => forall ctx (WF: URA.wf (fmr ⋅ ctx)),
                exists fmr0, URA.wf (fmr0 ⋅ ctx) /\ P fmr0.
 
-  Variant _hpsim'' {with_dummy safe_only: bool}
-    (hpsimc hpsimi: forall R (RR: Any.t * R -> Any.t * R -> iProp), bool -> bool -> Any.t * itree hAGEs R -> Any.t * itree hAGEs R -> Σ -> Prop)
-    {R} {RR: Any.t * R -> Any.t * R -> iProp}
+  Variant _hpsim' {with_dummy safe_only: bool}
+    (hpsimc: forall R (RR: Any.t * R -> Any.t * R -> iProp), bool -> bool -> Any.t * itree hAGEs R -> Any.t * itree hAGEs R -> Σ -> Prop)
+    {R} {RR: Any.t * R -> Any.t * R -> iProp} (hpsimi: bool -> bool -> Any.t * itree hAGEs R -> Any.t * itree hAGEs R -> Σ -> Prop)
     : bool -> bool -> Any.t * itree hAGEs R -> Any.t * itree hAGEs R -> Σ -> Prop := 
   | hpsim_ret
       (* Note: (INV: Own fmr ⊢ #=> Ist st_src st_tgt) is required only for the funtion end. *)
@@ -43,7 +68,7 @@ Section HPSIM.
       ps pt st_src st_tgt fmr v_src v_tgt
       (K: Own fmr ⊢ RR (st_src,v_src) (st_tgt,v_tgt))
     :
-    _hpsim'' hpsimc hpsimi ps pt (st_src, Ret v_src) (st_tgt, Ret v_tgt) fmr
+    _hpsim' hpsimc hpsimi ps pt (st_src, Ret v_src) (st_tgt, Ret v_tgt) fmr
 
   | hpsim_call
       (HPSIM_CALL: True)
@@ -51,113 +76,113 @@ Section HPSIM.
       (K: exists FR, (Own fmr ⊢ (Ist st_src st_tgt ** FR)) /\
           forall vret st_src0 st_tgt0 fmr' (* (WF: URA.wf fmr') *)
                  (INV: Own fmr' ⊢ (Ist st_src0 st_tgt0 ** FR)),
-          hpsimi R RR true true (st_src0, k_src vret) (st_tgt0, k_tgt vret) fmr')
+          hpsimi true true (st_src0, k_src vret) (st_tgt0, k_tgt vret) fmr')
     :
-    _hpsim'' hpsimc hpsimi ps pt (st_src, trigger (Call fn varg) >>= k_src) (st_tgt, trigger (Call fn varg) >>= k_tgt) fmr
+    _hpsim' hpsimc hpsimi ps pt (st_src, trigger (Call fn varg) >>= k_src) (st_tgt, trigger (Call fn varg) >>= k_tgt) fmr
 
   | hpsim_syscall
       (HPSIM_SYSCALL: True)
       ps pt st_src st_tgt fn varg rvs k_src k_tgt fmr 
       (K: forall vret, 
-          hpsimi R RR true true (st_src, k_src vret) (st_tgt, k_tgt vret) fmr)
+          hpsimi true true (st_src, k_src vret) (st_tgt, k_tgt vret) fmr)
     :
-    _hpsim'' hpsimc hpsimi ps pt (st_src, trigger (Syscall fn varg rvs) >>= k_src) (st_tgt, trigger (Syscall fn varg rvs) >>= k_tgt) fmr
+    _hpsim' hpsimc hpsimi ps pt (st_src, trigger (Syscall fn varg rvs) >>= k_src) (st_tgt, trigger (Syscall fn varg rvs) >>= k_tgt) fmr
 
   | hpsim_inline_src
       (HPSIM_INLINE_SRC: True)
       (NOTSAFE: negb safe_only)
       ps pt st_src st_tgt fn f varg k_src i_tgt fmr
       (FUN: alist_find fn fl_src = Some f)
-      (K: hpsimi R RR true pt (st_src, f varg >>= (if with_dummy then (fun x => trigger (Guarantee True) ;;; trigger (Assume True) ;;; k_src x) else k_src)) (st_tgt, i_tgt) fmr)
+      (K: hpsimi true pt (st_src, f varg >>= (if with_dummy then (fun x => trigger (Guarantee True) ;;; trigger (Assume True) ;;; k_src x) else k_src)) (st_tgt, i_tgt) fmr)
     :
-    _hpsim'' hpsimc hpsimi ps pt (st_src, trigger (Call fn varg) >>= k_src) (st_tgt, i_tgt) fmr
+    _hpsim' hpsimc hpsimi ps pt (st_src, trigger (Call fn varg) >>= k_src) (st_tgt, i_tgt) fmr
 
   | hpsim_inline_tgt
       (HPSIM_INLINE_TGT: True)
       (NOTSAFE: negb safe_only)
       ps pt st_src st_tgt fn f varg i_src k_tgt fmr
       (FUN: alist_find fn fl_tgt = Some f)
-      (K: hpsimi R RR ps true (st_src, i_src) (st_tgt, f varg >>= (if with_dummy then (fun x => trigger (Guarantee True) ;;; trigger (Assume True) ;;; k_tgt x) else k_tgt)) fmr)
+      (K: hpsimi ps true (st_src, i_src) (st_tgt, f varg >>= (if with_dummy then (fun x => trigger (Guarantee True) ;;; trigger (Assume True) ;;; k_tgt x) else k_tgt)) fmr)
     :
-    _hpsim'' hpsimc hpsimi ps pt (st_src, i_src) (st_tgt, trigger (Call fn varg) >>= k_tgt) fmr
+    _hpsim' hpsimc hpsimi ps pt (st_src, i_src) (st_tgt, trigger (Call fn varg) >>= k_tgt) fmr
 
   | hpsim_tau_src
       (HPSIM_TAU_SRC: True)
       ps pt st_src st_tgt i_src i_tgt fmr
-      (K: hpsimi R RR true pt (st_src, i_src) (st_tgt, i_tgt) fmr)
+      (K: hpsimi true pt (st_src, i_src) (st_tgt, i_tgt) fmr)
     :
-    _hpsim'' hpsimc hpsimi ps pt (st_src, tau;; i_src) (st_tgt, i_tgt) fmr
+    _hpsim' hpsimc hpsimi ps pt (st_src, tau;; i_src) (st_tgt, i_tgt) fmr
 
   | hpsim_tau_tgt
       (HPSIM_TAU_TGT: True)
       ps pt st_src st_tgt i_src i_tgt fmr
-      (K: hpsimi R RR ps true (st_src, i_src) (st_tgt, i_tgt) fmr)
+      (K: hpsimi ps true (st_src, i_src) (st_tgt, i_tgt) fmr)
     :
-    _hpsim'' hpsimc hpsimi ps pt (st_src, i_src) (st_tgt, tau;; i_tgt) fmr
+    _hpsim' hpsimc hpsimi ps pt (st_src, i_src) (st_tgt, tau;; i_tgt) fmr
 
   | hpsim_take_src
       (HPSIM_TAKE_SRC: True)
       ps pt st_src st_tgt X k_src i_tgt fmr
-      (K: forall (x: X), hpsimi R RR true pt (st_src, k_src x) (st_tgt, i_tgt) fmr)
+      (K: forall (x: X), hpsimi true pt (st_src, k_src x) (st_tgt, i_tgt) fmr)
     :
-    _hpsim'' hpsimc hpsimi ps pt (st_src, trigger (Take X) >>= k_src) (st_tgt, i_tgt) fmr
+    _hpsim' hpsimc hpsimi ps pt (st_src, trigger (Take X) >>= k_src) (st_tgt, i_tgt) fmr
 
   | hpsim_choose_tgt
       (HPSIM_CHOOSE_TGT: True)
       ps pt st_src st_tgt X i_src k_tgt fmr
-      (K: forall (x: X), hpsimi R RR ps true (st_src, i_src) (st_tgt, k_tgt x) fmr)
+      (K: forall (x: X), hpsimi ps true (st_src, i_src) (st_tgt, k_tgt x) fmr)
     :
-    _hpsim'' hpsimc hpsimi ps pt (st_src, i_src) (st_tgt, trigger (Choose X) >>= k_tgt) fmr
+    _hpsim' hpsimc hpsimi ps pt (st_src, i_src) (st_tgt, trigger (Choose X) >>= k_tgt) fmr
 
   | hpsim_choose_src
       (HPSIM_CHOOSE_SRC: True)
       (NOTSAFE: negb safe_only)
       ps pt st_src st_tgt X k_src i_tgt fmr
-      (K: exists x, hpsimi R RR true pt (st_src, k_src x) (st_tgt, i_tgt) fmr)
+      (K: exists x, hpsimi true pt (st_src, k_src x) (st_tgt, i_tgt) fmr)
     :
-    _hpsim'' hpsimc hpsimi ps pt (st_src, trigger (Choose X) >>= k_src) (st_tgt, i_tgt) fmr
+    _hpsim' hpsimc hpsimi ps pt (st_src, trigger (Choose X) >>= k_src) (st_tgt, i_tgt) fmr
 
   | hpsim_take_tgt
       (HPSIM_TAKE_TGT: True)
       (NOTSAFE: negb safe_only)
       ps pt st_src st_tgt X i_src k_tgt fmr
-      (K: exists x, hpsimi R RR ps true (st_src, i_src) (st_tgt, k_tgt x) fmr)
+      (K: exists x, hpsimi ps true (st_src, i_src) (st_tgt, k_tgt x) fmr)
     :
-    _hpsim'' hpsimc hpsimi ps pt (st_src, i_src) (st_tgt, trigger (Take X) >>= k_tgt) fmr
+    _hpsim' hpsimc hpsimi ps pt (st_src, i_src) (st_tgt, trigger (Take X) >>= k_tgt) fmr
 
   | hpsim_supdate_src
       (HPSIM_SUPDATE_SRC: True)
       ps pt st_src st_tgt X (run: Any.t -> Any.t * X) st_src0 x k_src i_tgt fmr
       (RUN: run st_src = (st_src0, x))      
-      (K: hpsimi R RR true pt (st_src0, k_src x) (st_tgt, i_tgt) fmr)
+      (K: hpsimi true pt (st_src0, k_src x) (st_tgt, i_tgt) fmr)
     :
-    _hpsim'' hpsimc hpsimi ps pt (st_src, trigger (SUpdate run) >>= k_src) (st_tgt, i_tgt) fmr
+    _hpsim' hpsimc hpsimi ps pt (st_src, trigger (SUpdate run) >>= k_src) (st_tgt, i_tgt) fmr
 
   | hpsim_supdate_tgt
       (HPSIM_SUPDATE_TGT: True)
       ps pt st_src st_tgt X (run: Any.t -> Any.t * X) st_tgt0 x i_src k_tgt fmr
       (RUN: run st_tgt = (st_tgt0, x))
-      (K: hpsimi R RR ps true (st_src, i_src) (st_tgt0, k_tgt x) fmr)
+      (K: hpsimi ps true (st_src, i_src) (st_tgt0, k_tgt x) fmr)
     :
-    _hpsim'' hpsimc hpsimi ps pt (st_src, i_src) (st_tgt, trigger (SUpdate run) >>= k_tgt) fmr
+    _hpsim' hpsimc hpsimi ps pt (st_src, i_src) (st_tgt, trigger (SUpdate run) >>= k_tgt) fmr
 
   | hpsim_assume_src
       (HPSIM_ASSUME_SRC: True)
       ps pt st_src st_tgt iP k_src i_tgt fmr
       (K: forall fmr' (* (WF: URA.wf fmr') *)
                  (NEW: Own fmr' ⊢ (iP ** Own fmr)),
-          hpsimi R RR true pt (st_src, k_src tt) (st_tgt, i_tgt) fmr')
+          hpsimi true pt (st_src, k_src tt) (st_tgt, i_tgt) fmr')
     :
-    _hpsim'' hpsimc hpsimi ps pt (st_src, trigger (Assume iP) >>= k_src) (st_tgt, i_tgt) fmr
+    _hpsim' hpsimc hpsimi ps pt (st_src, trigger (Assume iP) >>= k_src) (st_tgt, i_tgt) fmr
 
   | hpsim_guarantee_tgt
       (HPSIM_GUARANTEE_TGT: True)
       ps pt st_src st_tgt iP i_src k_tgt fmr
       (K: forall fmr' (* (WF: URA.wf fmr') *)
                  (NEW: Own fmr' ⊢ (iP ** Own fmr)),
-          hpsimi R RR ps true (st_src, i_src) (st_tgt, k_tgt tt) fmr')
+          hpsimi ps true (st_src, i_src) (st_tgt, k_tgt tt) fmr')
     :
-    _hpsim'' hpsimc hpsimi ps pt (st_src, i_src) (st_tgt, trigger (Guarantee iP) >>= k_tgt) fmr
+    _hpsim' hpsimc hpsimi ps pt (st_src, i_src) (st_tgt, trigger (Guarantee iP) >>= k_tgt) fmr
 
   | hpsim_guarantee_src
       (HPSIM_GUARANTEE_SRC: True)
@@ -166,9 +191,9 @@ Section HPSIM.
       (K: exists FMR, (Own fmr ⊢ iP ** FMR) /\
           forall fmr' (* (WF: URA.wf fmr') *)
                  (NEW: Own fmr' ⊢ FMR),
-            hpsimi R RR true pt (st_src, k_src tt) (st_tgt, i_tgt) fmr')
+            hpsimi true pt (st_src, k_src tt) (st_tgt, i_tgt) fmr')
     :
-    _hpsim'' hpsimc hpsimi ps pt (st_src, trigger (Guarantee iP) >>= k_src) (st_tgt, i_tgt) fmr
+    _hpsim' hpsimc hpsimi ps pt (st_src, trigger (Guarantee iP) >>= k_src) (st_tgt, i_tgt) fmr
 
   | hpsim_assume_tgt
       (HPSIM_ASSUME_TGT: True)
@@ -177,9 +202,9 @@ Section HPSIM.
       (K: exists FMR, (Own fmr ⊢ iP ** FMR) /\
           forall fmr' (* (WF: URA.wf fmr') *)
                  (NEW: Own fmr' ⊢ FMR),
-          hpsimi R RR ps true (st_src, i_src) (st_tgt, k_tgt tt) fmr')
+          hpsimi ps true (st_src, i_src) (st_tgt, k_tgt tt) fmr')
     :
-    _hpsim'' hpsimc hpsimi ps pt (st_src, i_src) (st_tgt, trigger (Assume iP) >>= k_tgt) fmr
+    _hpsim' hpsimc hpsimi ps pt (st_src, i_src) (st_tgt, trigger (Assume iP) >>= k_tgt) fmr
 
   | hpsim_progress
       (HPSIM_PROGRESS: True)
@@ -187,47 +212,58 @@ Section HPSIM.
       sti_src sti_tgt fmr
       (K: hpsimc R RR false false sti_src sti_tgt fmr)
     :
-    _hpsim'' hpsimc hpsimi true true sti_src sti_tgt fmr
+    _hpsim' hpsimc hpsimi true true sti_src sti_tgt fmr
   .
-  Arguments _hpsim'' with_dummy safe_only hpsimc hpsimi R RR.
+  Arguments _hpsim' with_dummy safe_only hpsimc R RR hpsimi.
 
-  Definition _hpsim' with_dummy safe_only hpsimc hpsimi R RR ps pt sti_src sti_tgt :=
-    hsupd (@_hpsim'' with_dummy safe_only hpsimc hpsimi R RR ps pt sti_src sti_tgt).
+  (* Definition _hpsim' with_dummy safe_only hpsimc hpsimi R RR ps pt sti_src sti_tgt := *)
+  (*   hsupd (@_hpsim' with_dummy safe_only hpsimc hpsimi R RR ps pt sti_src sti_tgt). *)
 
   Inductive _hpsim {with_dummy} hpsim R RR ps pt sti_src sti_tgt fmr : Prop
     :=
-  | hpsimF_intro (IN: @_hpsim' with_dummy false hpsim (@_hpsim with_dummy hpsim) R RR ps pt sti_src sti_tgt fmr) 
+  | hpsimF_intro (IN: hsupd (@_hpsim' with_dummy false hpsim R RR (@_hpsim with_dummy hpsim R RR) ps pt sti_src sti_tgt) fmr) 
   .
   
   Definition hpsim {R} RR := paco7 (@_hpsim false) bot7 R RR.
 
-  Lemma _hpsim_tarski with_dummy hpsim rel
-    (FIX: @_hpsim' with_dummy false hpsim rel <7= rel)
+  Lemma _hpsim_tarski with_dummy hpsim R RR rel
+    (FIX: forall ps pt sti_src sti_tgt fmr
+            (IN: hsupd (@_hpsim' with_dummy false hpsim R RR rel ps pt sti_src sti_tgt) fmr),
+          rel ps pt sti_src sti_tgt fmr)
     :
-    @_hpsim with_dummy hpsim <7= rel.
+    @_hpsim with_dummy hpsim R RR <5= rel.
   Proof.
-    fix self 8. i.
+    fix self 6. i.
     destruct PR. apply FIX.
     ii. exploit IN; eauto. i; des.
-    destruct x8; des; esplits; eauto; econs; esplits; eauto.
+    destruct x6; des; esplits; eauto; econs; esplits; eauto.
   Qed.
 
+  Lemma hsupd_mon P Q r
+    (IN: hsupd P r)             
+    (LE: P <1= Q)
+    :
+    hsupd Q r.
+  Proof.
+    unfold hsupd in *; i. exploit IN; eauto.
+    i; des. esplits; eauto.
+  Qed.
+  
   Lemma _hpsim'_mon with_dummy safe_only r r' R RR s s'
     ps pt sti_src sti_tgt fmr
-    (REL: @_hpsim' with_dummy safe_only r s R RR ps pt sti_src sti_tgt fmr)
+    (REL: @_hpsim' with_dummy safe_only r R RR s ps pt sti_src sti_tgt fmr)
     (LEr: r <7= r')
-    (LEs: s <7= s')
+    (LEs: s <5= s')
     :
-    @_hpsim' with_dummy safe_only r' s' R RR ps pt sti_src sti_tgt fmr.
+    @_hpsim' with_dummy safe_only r' R RR s' ps pt sti_src sti_tgt fmr.
   Proof.
-    ii. exploit REL; eauto. i; des.
-    destruct x1; des; esplits; eauto; econs; esplits; eauto.
+    ii. destruct REL; des; esplits; eauto; econs; esplits; eauto.
   Qed.
 
   Lemma _hpsim_mon with_dummy: monotone7 (@_hpsim with_dummy).
   Proof. 
     ii. eapply _hpsim_tarski, IN.
-    i. econs. eapply _hpsim'_mon; eauto.
+    i. econs. eauto using hsupd_mon, _hpsim'_mon.
   Qed.
 
   Lemma _hpsim_mon_auto with_dummy r r' R RR
@@ -238,11 +274,10 @@ Section HPSIM.
     @_hpsim with_dummy r' R RR ps pt sti_src sti_tgt fmr.
   Proof. eapply _hpsim_mon; eauto. Qed.
   
-  Hint Constructors _hpsim'' _hpsim.
-  Hint Unfold _hpsim' hpsim.
-  Hint Resolve _hpsim'_mon: paco.
+  Hint Constructors _hpsim' _hpsim.
+  Hint Unfold hpsim.
   Hint Resolve _hpsim_mon: paco.
-  Hint Resolve _hpsim_mon_auto: paco.
+  Hint Resolve hsupd_mon _hpsim'_mon _hpsim_mon_auto: paco.
   Hint Resolve cpn7_wcompat: paco.
 
   Definition hpsim_tail : Any.t*Any.t -> Any.t*Any.t -> iProp :=
@@ -280,15 +315,6 @@ Section HPSIM.
       repeat f_equal. extensionality x. rewrite bind_ret_l. eauto.
   Qed.
 
-  Lemma hsupd_mon P Q
-    (LE: P <1= Q)
-    :
-    hsupd P <1= hsupd Q.
-  Proof.
-    unfold hsupd; i. exploit PR; eauto.
-    i; des. esplits; eauto.
-  Qed.
-
   Lemma hsupd_incl P
     :
     P <1= hsupd P.
@@ -305,15 +331,6 @@ Section HPSIM.
     specialize (REL0 _ REL). des. eauto.
   Qed.
   
-  Lemma _hpsim'_upd
-    with_dummy safe_only hpsimc hpsimi R RR ps pt sti_src sti_tgt (fmr: Σ)
-    (K: hsupd (@_hpsim' with_dummy safe_only hpsimc hpsimi R RR ps pt sti_src sti_tgt) fmr)
-    :
-    @_hpsim' with_dummy safe_only hpsimc hpsimi R RR ps pt sti_src sti_tgt fmr.
-  Proof.
-    eapply hsupd_merge. eauto.
-  Qed.
-
   Lemma _hpsim_flag_mon r R RR (ps pt ps' pt': bool) st_src st_tgt fmr
     (SIM: @_hpsim false r R RR ps pt st_src st_tgt fmr)
     (LES: ps -> ps')
@@ -322,10 +339,10 @@ Section HPSIM.
     @_hpsim false r R RR ps' pt' st_src st_tgt fmr.
   Proof.
     move SIM before r. revert_until SIM.
-    pattern R, RR, ps, pt, st_src, st_tgt, fmr.
+    pattern ps, pt, st_src, st_tgt, fmr.
     eapply _hpsim_tarski, SIM. i. econs.
-    ii. exploit PR; eauto. i; des.
-    destruct x8; des; esplits; eauto; try by econs; esplits; eauto.
+    ii. exploit IN; eauto. i; des.
+    destruct x1; des; esplits; eauto; try by econs; esplits; eauto.
     hexploit LES; eauto; i. hexploit LET; eauto; i.
     destruct ps', pt'; try discriminate. 
     econs; esplits; eauto.
@@ -377,10 +394,10 @@ Section HPSIM.
     eapply wrespect7_uclo; eauto with paco.
     econs; eauto with paco. i. inv PR.
     eapply GF in SIM.
-    move SIM before GF. revert_until SIM. pattern x0, x1, ps0, pt0, x4, x5, x6.
+    move SIM before GF. revert_until SIM. pattern ps0, pt0, x4, x5, x6.
     eapply _hpsim_tarski, SIM. econs.
-    ii. exploit PR; eauto. i; des.
-    destruct x15; des; esplits; eauto; try by econs; esplits; eauto.
+    ii. exploit IN; eauto. i; des.
+    destruct x8; des; esplits; eauto; try by econs; esplits; eauto.
     exploit SRC; et. exploit TGT; et. i; clarify.
     econs; esplits; eauto using rclo7.
   Qed.
@@ -396,8 +413,8 @@ Section HPSIM.
 
 
 
-  Definition hpsimC with_dummy hpsim :=
-    @_hpsim' with_dummy false hpsim hpsim.
+  Definition hpsimC with_dummy hpsim R RR ps pt sti_src sti_tgt fmr :=
+    hsupd (@_hpsim' with_dummy false hpsim R RR (hpsim R RR) ps pt sti_src sti_tgt) fmr.
   
   Lemma hpsimC_mon with_dummy : monotone7 (@hpsimC with_dummy).
   Proof.
@@ -418,8 +435,8 @@ Section HPSIM.
 
 
 
-  Definition safe_hpsim hpsim :=
-    @_hpsim' false true hpsim hpsim.
+  Definition safe_hpsim hpsim R RR ps pt sti_src sti_tgt fmr :=
+    hsupd (@_hpsim' false true hpsim R RR (hpsim R RR) ps pt sti_src sti_tgt) fmr.
 
   Lemma safe_hpsim_spec:
     safe_hpsim <8= gupaco7 (@_hpsim false) (cpn7 (@_hpsim false)).
@@ -466,9 +483,9 @@ Section HPSIM.
     remember (st_src, i_src) as sti_src. remember (st_tgt, i_tgt) as sti_tgt.
     move SIM before GF. revert_until SIM.
     pattern Q, QQ, ps, pt, sti_src, sti_tgt, fmr.
-    eapply _hpsim_tarski, SIM. econs. apply _hpsim'_upd.
-    ii. exploit PR; eauto. i; des.
-    destruct x8; des; depdes Heqsti_src Heqsti_tgt; grind; esplits;
+    eapply _hpsim_tarski, SIM. econs. apply hsupd_merge.
+    ii. exploit IN; eauto. i; des.
+    destruct x1; des; depdes Heqsti_src Heqsti_tgt; grind; esplits;
       try by ii; esplits; eauto with paco.
     - hexploit SIMK; eauto. i. apply GF in H.
       eapply _hpsim_mon.
@@ -492,19 +509,6 @@ Section HPSIM.
 
 
   
-  Lemma URA_wf_extends_add (r r' c: Σ)
-    (EXT : URA.extends r r')
-    (WF : URA.wf (r' ⋅ c))
-    :
-    URA.wf (r ⋅ c).
-  Proof.
-    eapply URA.wf_extends; eauto.
-    eapply URA.extends_add. eauto.
-  Qed.
-
-  Lemma URA_extends_refl (r: Σ):
-    URA.extends r r.
-  Proof. refl. Qed.
 
 
 
@@ -536,8 +540,8 @@ Section HPSIM.
     intros. destruct PR. move SIM before r. revert_until SIM.
     pattern R, RR, ps, pt, sti_src, sti_tgt, fmr.
     eapply _hpsim_tarski, SIM. econs.
-    ii. exploit PR; eauto using URA_wf_extends_add. i; des.
-    destruct x8; des; grind; esplits; eauto using hpsim_extendC, URA_extends_refl;
+    ii. exploit IN; eauto using URA_wf_extends_add. i; des.
+    destruct x1; des; grind; esplits; eauto using hpsim_extendC, URA_extends_refl;
       econs; rr; esplits; i; eauto;
       try by try eapply K; try eapply K0; eauto; try refl.
   Qed.
@@ -578,11 +582,10 @@ Section HPSIM.
     compatible7 (@_hpsim false) hpsim_updateC.
   Proof.
     econs; eauto using hpsim_updateC_mon.
-    i. destruct PR. econs. eapply _hpsim'_upd.
-    eapply hsupd_mon, EXT.
+    i. destruct PR. econs. eapply hsupd_merge.
+    eapply hsupd_mon; eauto.
     i. destruct PR.
-    eapply _hpsim'_mon; eauto using hpsim_updateC, hsupd_incl.
-    i. eapply _hpsim_mon; eauto using hpsim_updateC, hsupd_incl.
+    eauto 10 using hpsim_updateC, hsupd_incl with paco.
   Qed.
   
   Lemma hpsim_updateC_spec:
@@ -628,9 +631,8 @@ Section HPSIM.
     i. destruct PR. econs. ii.
     exploit EXT.
     { eapply URA.wf_mon; eauto. }
-    i. destruct x0. eapply _hpsim'_mon in IN; eauto.
-    - eauto using hpsim_wfC.
-    - i. eapply _hpsim_mon; eauto using hpsim_wfC.
+    i. destruct x0. edestruct IN; eauto. des.
+    eauto 10 using hpsim_wfC, hsupd_incl with paco.
   Qed.
   
   Lemma hpsim_wfC_spec:
@@ -642,295 +644,6 @@ Section HPSIM.
 
 
   
-(*
-  Definition itreeH_dummy_ktree R (k k': R -> itree hAGEs Any.t) :=
-    k' = k \/ k' = (fun x => trigger (Guarantee True);;; trigger (Assume True);;; k x).
-  Hint Unfold itreeH_dummy_ktree.
-  
-  Definition itreeH_dummy (itr itr': itree hAGEs Any.t) :=
-    exists R i k k',
-      itr = (i >>= k) /\
-      itr' = (i >>= k') /\
-      itreeH_dummy_ktree R k k'.
-  Hint Unfold itreeH_dummy.
-
-  Lemma itreeH_dummy_refl i:
-    itreeH_dummy i i.
-  Proof.
-    replace i with (x <- Ret tt;; Ret tt;;; i); cycle 1.
-    { rewrite !bind_ret_l. eauto. }
-    r; esplits; last left; eauto; grind.
-  Qed.
-  Hint Resolve itreeH_dummy_refl.
-  
-  Lemma itreeH_dummy_dummy R i (k: R -> _):
-    itreeH_dummy (i >>= k) (x <- i ;; trigger (Guarantee True);;; trigger (Assume True);;; k x).
-  Proof.
-    r; esplits; last right; eauto.
-  Qed.
-  Hint Resolve itreeH_dummy_dummy.
-
-  Variant hpsim_dummyC_src (r: forall R (RR: Any.t * R -> Any.t * R -> Σ -> iProp), bool -> bool -> Any.t * itree hAGEs R -> Any.t * itree hAGEs R -> Σ -> Σ -> Prop):
-    forall R (RR: Any.t * R -> Any.t * R -> Σ -> iProp), bool -> bool -> Any.t * itree hAGEs R -> Any.t * itree hAGEs R -> Σ -> Σ -> Prop
-  :=
-  | hpsim_dummyC_src_intro ps pt st_src i_src i_src' st_tgt i_tgt ctx fmr fmr'
-      (SIM: r _ hpsim_tail ps pt (st_src, i_src) (st_tgt, i_tgt) ctx fmr)
-      (RELr: Own fmr' ⊢ Own fmr)
-      (WF: URA.wf (fmr' ⋅ ctx))
-      (DUMMY: itreeH_dummy i_src i_src')
-    :
-    hpsim_dummyC_src r _ hpsim_tail ps pt (st_src, i_src') (st_tgt, i_tgt) ctx fmr'
-  .
-  
-  Lemma hpsim_dummyC_src_mon
-        r1 r2
-        (LEr: r1 <7= r2)
-    :
-    hpsim_dummyC_src r1 <7= hpsim_dummyC_src r2
-  .
-  Proof. i. destruct PR; econs; eauto. Qed.
-
-  Lemma hpsim_dummyC_src_compatible with_dummy:
-    compatible7 (@_hpsim with_dummy) hpsim_dummyC_src.
-  Proof.
-    econs; eauto using hpsim_dummyC_src_mon; i. depdes PR.
-    remember (st_src, i_src) as sti_src.
-    remember (st_tgt, i_tgt) as sti_tgt.
-    move SIM before r. revert_until SIM.
-    induction SIM; i; depdes Heqsti_src Heqsti_tgt;
-      grind; eauto 7 with paco; r in DUMMY; des.
-    - assert (CASE:= case_itrH _ i); des; subst; itree_clarify DUMMY.
-      destruct DUMMY1; subst; rewrite <-x; eauto.
-      + econs; eauto. etrans; eauto.
-      + econs; try (instantiate (1:=ε)); eauto.
-        { r_solve. rewrite URA.add_comm in WF. eapply URA.wf_mon; eauto. }
-        { instantiate (1:= Own ε). eauto. }
-        i. econs; eauto.
-        i. econs; eauto.
-        unfold hpsim_tail in *.
-        
-        iIntros "H". iPoseProof (NEW0 with "H") as "[_ H]".
-        
-        
-
-      
-        
-
-        
-    - assert (CASE:= case_itrH _ i); des; subst; itree_clarify DUMMY.
-
-      
-      + destruct DUMMY1; subst; rewrite -x -(bind_ret_l_eta _ k_src) -bind_vis.
-        * econs; eauto with imodL.
-        * eapply hpsim_guarantee_src; try econs; eauto with imodL.
-      + replace c with (Call fn varg).
-        econs; eauto with imodL.
-        i. destruct DUMMY1; subst; eauto with imodL.
-    - assert (CASE:= case_itrH _ i); des; subst; itree_clarify DUMMY.
-      + destruct DUMMY1; subst; rewrite -x -(bind_ret_l_eta _ k_src) -bind_vis.
-        * econs; eauto.
-        * eapply hpsim_guarantee_src; try econs; eauto with imodL.
-      + replace e with (Syscall fn varg rvs).
-        econs; eauto with imodL.
-        i. destruct DUMMY1; subst; eauto with imodL.
-    - assert (CASE:= case_itrH _ i); des; subst; itree_clarify DUMMY.
-      + destruct DUMMY1; subst; rewrite -x -(bind_ret_l_eta _ k_src) -bind_vis.
-        * econs; eauto.
-        * eapply hpsim_guarantee_src; try econs; eauto with imodL.
-      + replace c with (Call fn varg).
-        econs; eauto with imodL.
-        destruct DUMMY1; subst; destruct with_dummy; eauto.
-        * eapply IHSIM; eauto.
-          eexists _, (x<-f varg;; trigger (Guarantee True);;; ktrH' x), k, _.
-          esplits; eauto; grind.
-        * eapply IHSIM; eauto.
-          eexists _, (f varg >>= ktrH'), k, _.
-          esplits; eauto; grind.
-    - assert (CASE:= case_itrH _ i); des; subst; itree_clarify DUMMY.
-      + destruct DUMMY1; subst; rewrite -x; eauto.
-        eapply hpsim_guarantee_src; eauto with imodL.
-      + econs; eauto with imodL.
-        destruct DUMMY1; subst; eauto with imodL.
-    - assert (CASE:= case_itrH _ i); des; subst; itree_clarify DUMMY.
-      + destruct DUMMY1; subst; rewrite -x -(bind_ret_l_eta _ k_src) -bind_vis.
-        * econs; eauto.
-        * eapply hpsim_guarantee_src; eauto with imodL.
-          econs; eauto with imodL.
-      + replace e with (Choose R0); econs; eauto.
-        i. destruct DUMMY1; subst; eauto.
-    - assert (CASE:= case_itrH _ i); des; subst; itree_clarify DUMMY.
-      + destruct DUMMY1; subst; rewrite -x -(bind_ret_l_eta _ k_src) -bind_vis.
-        * econs; eauto.
-        * eapply hpsim_guarantee_src; eauto with imodL.
-          econs; eauto with imodL.
-      + replace e with (Take R0); econs; eauto.
-        i. destruct DUMMY1; subst; eauto.
-    - assert (CASE:= case_itrH _ i); des; subst; itree_clarify DUMMY.
-      + destruct DUMMY1; subst; rewrite -x -(bind_ret_l_eta _ k_src) -bind_vis.
-        * econs; eauto.
-        * eapply hpsim_guarantee_src; eauto with imodL.
-          econs; eauto.
-      + replace s with (SUpdate run); econs; eauto.
-        i. destruct DUMMY1; subst; eauto.
-    - assert (CASE:= case_itrH _ i); des; subst; itree_clarify DUMMY.
-      + destruct DUMMY1; subst; rewrite -x -(bind_ret_l_eta _ k_src) -bind_vis.
-        * econs; try instantiate (1:=FMR); eauto with imodL.
-        * eapply hpsim_guarantee_src; eauto with imodL.
-          econs; try instantiate (1:=FMR); eauto with imodL.
-      + econs; eauto. i. eapply H; eauto.
-        { eapply imod_trans; eauto.
-          iIntros "H". iDestruct "H" as "[X H]".
-          iSplitL "X"; eauto. iStopProof; eauto. }
-        destruct DUMMY1; subst; eauto.
-    - assert (CASE:= case_itrH _ i); des; subst; itree_clarify DUMMY.
-      + destruct DUMMY1; subst; rewrite -x -(bind_ret_l_eta _ k_src) -bind_vis.
-        * econs; eauto with imodL.
-        * eapply hpsim_guarantee_src; eauto with imodL.
-          econs; eauto with imodL.
-      + econs; eauto with imodL.
-        i. eapply H; eauto. destruct DUMMY1; subst; eauto.
-    - subst. econs; eauto. destruct DUMMY1; subst; econs; eauto.
-  Qed.
-
-  Lemma hpsim_dummyC_src_spec (with_dummy:bool) :
-    hpsim_dummyC_src <8= gupaco7 (@_hpsim with_dummy) (cpn7 (@_hpsim with_dummy)).
-  Proof.
-    intros. gclo. econs; eauto using hpsim_dummyC_src_compatible.
-    eapply hpsim_dummyC_src_mon, PR; eauto with paco.
-  Qed.
-
-  Variant hpsim_dummyC_tgt (r: forall R (RR: Any.t * R -> Any.t * R -> iProp), bool -> bool -> Any.t * itree hAGEs R -> Any.t * itree hAGEs R -> Σ -> Prop):
-    forall R (RR: Any.t * R -> Any.t * R -> iProp), bool -> bool -> Any.t * itree hAGEs R -> Any.t * itree hAGEs R -> Σ -> Prop
-  :=
-  | hpsim_dummyC_tgt_intro R RR ps pt st_src i_src st_tgt i_tgt i_tgt' fmr fmr'
-      (SIM: r R RR ps pt (st_src, i_src) (st_tgt, i_tgt) fmr)
-      (RELr: Own fmr' ⊢ #=> Own fmr)
-      (DUMMY: itreeH_dummy R i_tgt i_tgt')
-    :
-    hpsim_dummyC_tgt r R RR ps pt (st_src, i_src) (st_tgt, i_tgt') fmr'
-  .
-  
-  Lemma hpsim_dummyC_tgt_mon
-        r1 r2
-        (LEr: r1 <7= r2)
-    :
-    hpsim_dummyC_tgt r1 <7= hpsim_dummyC_tgt r2
-  .
-  Proof. i. destruct PR; econs; eauto. Qed.
-
-  Lemma hpsim_dummyC_tgt_compatible with_dummy:
-    compatible7 (@_hpsim with_dummy) hpsim_dummyC_tgt.
-  Proof.
-    econs; eauto using hpsim_dummyC_tgt_mon; i. depdes PR.
-    remember (st_src, i_src) as sti_src.
-    remember (st_tgt, i_tgt) as sti_tgt.
-    move SIM before RR. revert_until SIM.
-    induction SIM; i; depdes Heqsti_src Heqsti_tgt;
-      grind; eauto 7 with paco imodL; r in DUMMY; des.
-    - assert (CASE:= case_itrH _ i); des; subst; itree_clarify DUMMY.
-      destruct DUMMY1; subst; rewrite <-x; econs; eauto; imodIntroL.
-    - assert (CASE:= case_itrH _ i); des; subst; itree_clarify DUMMY.
-      + destruct DUMMY1; subst; rewrite -x -(bind_ret_l_eta _ k_tgt) -bind_vis.
-        * econs; eauto with imodL.
-        * eapply hpsim_guarantee_tgt; try econs; eauto; imodIntroL.
-      + replace c with (Call fn varg).
-        econs; eauto with imodL.
-        i. destruct DUMMY1; subst; eauto with imodL.
-    - assert (CASE:= case_itrH _ i); des; subst; itree_clarify DUMMY.
-      + destruct DUMMY1; subst; rewrite -x -(bind_ret_l_eta _ k_tgt) -bind_vis.
-        * econs; eauto.
-        * eapply hpsim_guarantee_tgt; try econs; eauto; imodIntroL.
-      + replace e with (Syscall fn varg rvs).
-        econs; eauto with imodL.
-        i. destruct DUMMY1; subst; eauto with imodL.
-    - assert (CASE:= case_itrH _ i); des; subst; itree_clarify DUMMY.
-      + destruct DUMMY1; subst; rewrite -x -(bind_ret_l_eta _ k_tgt) -bind_vis.
-        * econs; eauto.
-        * eapply hpsim_guarantee_tgt; try econs; eauto; imodIntroL.
-      + replace c with (Call fn varg).
-        econs; eauto with imodL.
-        destruct DUMMY1; subst; destruct with_dummy; eauto.
-        * eapply IHSIM; eauto.
-          eexists _, (x<-f varg;; trigger (Guarantee True);;; ktrH' x), k, _.
-          esplits; eauto; grind.
-        * eapply IHSIM; eauto.
-          eexists _, (f varg >>= ktrH'), k, _.
-          esplits; eauto; grind.
-    - assert (CASE:= case_itrH _ i); des; subst; itree_clarify DUMMY.
-      + destruct DUMMY1; subst; rewrite -x; eauto.
-        eapply hpsim_guarantee_tgt; eauto; imodIntroL.
-      + econs; eauto with imodL.
-        destruct DUMMY1; subst; eauto with imodL.
-    - assert (CASE:= case_itrH _ i); des; subst; itree_clarify DUMMY.
-      + destruct DUMMY1; subst; rewrite -x -(bind_ret_l_eta _ k_tgt) -bind_vis.
-        * econs; eauto.
-        * eapply hpsim_guarantee_tgt; eauto with imodL.
-          econs; eauto; imodIntroL.
-      + replace e with (Choose R0); econs; eauto.
-        i. destruct DUMMY1; subst; eauto.
-    - assert (CASE:= case_itrH _ i); des; subst; itree_clarify DUMMY.
-      + destruct DUMMY1; subst; rewrite -x -(bind_ret_l_eta _ k_tgt) -bind_vis.
-        * econs; eauto.
-        * eapply hpsim_guarantee_tgt; eauto with imodL.
-          econs; eauto; imodIntroL.
-      + replace e with (Take R0); econs; eauto.
-        i. destruct DUMMY1; subst; eauto.
-    - assert (CASE:= case_itrH _ i); des; subst; itree_clarify DUMMY.
-      + destruct DUMMY1; subst; rewrite -x -(bind_ret_l_eta _ k_tgt) -bind_vis.
-        * econs; eauto.
-        * eapply hpsim_guarantee_tgt; eauto with imodL.
-          econs; eauto; imodIntroL.
-      + replace s with (SUpdate run); econs; eauto.
-        i. destruct DUMMY1; subst; eauto.
-    - assert (CASE:= case_itrH _ i); des; subst; itree_clarify DUMMY.
-      + destruct DUMMY1; subst; rewrite -x -(bind_ret_l_eta _ k_tgt) -bind_vis.
-        * econs; try instantiate (1:=FMR); eauto with imodL.
-        * eapply hpsim_guarantee_tgt; eauto with imodL.
-          econs; try instantiate (1:=FMR); eauto; imodIntroL.
-      + econs; eauto; imodIntroL. eapply H; eauto 10.
-    - assert (CASE:= case_itrH _ i); des; subst; itree_clarify DUMMY.
-      + destruct DUMMY1; subst; rewrite -x -(bind_ret_l_eta _ k_tgt) -bind_vis.
-        * econs; eauto. i. eapply H; eauto.
-          eapply imod_trans; eauto.
-          iIntros "H". iDestruct "H" as "[X H]".
-          iSplitL "X"; eauto. iStopProof; eauto.
-        * eapply hpsim_guarantee_tgt; eauto. econs; eauto.
-          i. eapply H; eauto.
-          iIntros "H". iPoseProof (NEW0 with "H") as "H". iMod "H".
-          iDestruct "H" as "[P [_ H]]". iSplitL "P"; eauto. iStopProof; eauto.
-      + econs; eauto with imodL.
-        i. eapply H; eauto.
-        { iIntros "H". iPoseProof (NEW with "H") as "H". iMod "H".
-          iDestruct "H" as "[P H]". iSplitL "P"; eauto. iStopProof; eauto. }
-        destruct DUMMY1; subst; eauto.
-    - subst. econs; eauto. destruct DUMMY1; subst; econs; eauto.
-  Qed.
-
-  Lemma hpsim_dummyC_tgt_spec (with_dummy:bool) :
-    hpsim_dummyC_tgt <8= gupaco7 (@_hpsim with_dummy) (cpn7 (@_hpsim with_dummy)).
-  Proof.
-    intros. gclo. econs; eauto using hpsim_dummyC_tgt_compatible.
-    eapply hpsim_dummyC_tgt_mon, PR; eauto with paco.
-  Qed.
-  
-  Lemma hpsim_le_gpaco with_dummy r r':
-    @hpsim <7= gpaco7 (@_hpsim with_dummy) (cpn7 (@_hpsim with_dummy)) r r'.
-  Proof.
-    gcofix CIH. i. punfold PR.
-    induction PR; pclearbot; eauto with paco;
-      guclo hpsimC_spec; eauto with paco.
-    - econs; eauto. destruct with_dummy; eauto.
-      guclo hpsim_dummyC_src_spec. econs; eauto.
-    - econs; eauto. destruct with_dummy; eauto.
-      guclo hpsim_dummyC_tgt_spec. econs; eauto.
-  Qed.
-  
-  Hint Resolve hpsim_le_gpaco: paco.
-
-  Corollary hpsim_add_dummy:
-    @hpsim <7= paco7 (@_hpsim true) bot7.
-  Proof. ginit. eauto with paco. Qed.
-*)
 
   Definition hpsim_fsem: relation (Any.t -> itree hAGEs Any.t) :=
     (eq ==> hpsim_fun)%signature.
